Work towards proper guards for well-formedness of SMT types  (#25)
* Another attempt at setting up well-formedness of type

* No nested recursion

* Fixes

* Another

* Inhabited issues

* More

* Guard selector

* Fix proofs

* Fixing, changes smt model

* Revert

* Repair again, possibly infeasible dt sorry for now

* Fix

Cpc/SmtModel.lean
@@ -387,9 +387,11 @@ inductive SmtValue : Type where
   | Rational : native_Rat -> SmtValue
   | Binary : native_Int -> native_Int -> SmtValue
   | Map : SmtMap -> SmtValue
+  | Fun : SmtMap -> SmtValue
   | Set : SmtMap -> SmtValue
   | Seq : SmtSeq -> SmtValue
   | Char : native_Char -> SmtValue
+  | UValue : native_Nat -> native_Nat -> SmtValue
   | RegLan : native_RegLan -> SmtValue
   | DtCons : native_String -> SmtDatatype -> native_Nat -> SmtValue
   | Apply : SmtValue -> SmtValue -> SmtValue
@@ -549,6 +551,7 @@ def __vsm_apply_arg_nth : SmtValue -> native_Nat -> native_Nat -> SmtValue
 
 
 def __smtx_dt_cons_wf_rec : SmtDatatypeCons -> RefList -> native_Bool
+  | (SmtDatatypeCons.cons (SmtType.TypeRef s) c), refs => (native_ite (native_reflist_contains refs s) (__smtx_dt_cons_wf_rec c refs) false)
   | (SmtDatatypeCons.cons T c), refs => (native_ite (__smtx_type_wf_rec T refs) (__smtx_dt_cons_wf_rec c refs) false)
   | SmtDatatypeCons.unit, refs => true
 
@@ -560,11 +563,11 @@ def __smtx_dt_wf_rec : SmtDatatype -> RefList -> native_Bool
 
 def __smtx_type_wf_rec : SmtType -> RefList -> native_Bool
   | (SmtType.Datatype s d), refs => (__smtx_dt_wf_rec d (native_reflist_insert refs s))
-  | (SmtType.TypeRef s), refs => (native_reflist_contains refs s)
-  | (SmtType.Seq x1), refs => (__smtx_type_wf_rec x1 refs)
-  | (SmtType.Map x1 x2), refs => (native_and (__smtx_type_wf_rec x1 refs) (__smtx_type_wf_rec x2 refs))
-  | (SmtType.FunType x1 x2), refs => (native_and (__smtx_type_wf_rec x1 refs) (__smtx_type_wf_rec x2 refs))
-  | (SmtType.Set x1), refs => (__smtx_type_wf_rec x1 refs)
+  | (SmtType.TypeRef s), refs => false
+  | (SmtType.Seq x1), refs => (__smtx_type_wf_rec x1 native_reflist_nil)
+  | (SmtType.Map x1 x2), refs => (native_and (__smtx_type_wf_rec x1 native_reflist_nil) (__smtx_type_wf_rec x2 native_reflist_nil))
+  | (SmtType.FunType x1 x2), refs => (native_and (__smtx_type_wf_rec x1 native_reflist_nil) (__smtx_type_wf_rec x2 native_reflist_nil))
+  | (SmtType.Set x1), refs => (__smtx_type_wf_rec x1 native_reflist_nil)
   | SmtType.None, refs => false
   | T, refs => true
 
@@ -575,11 +578,8 @@ def __smtx_type_wf (T : SmtType) : native_Bool :=
 def __smtx_typeof_guard (T : SmtType) (U : SmtType) : SmtType :=
   (native_ite (native_Teq T SmtType.None) SmtType.None U)
 
-def __smtx_typeof_guard_inhabited (T : SmtType) (U : SmtType) : SmtType :=
-  (native_ite (native_inhabited_type T) U SmtType.None)
-
 def __smtx_typeof_guard_wf (T : SmtType) (U : SmtType) : SmtType :=
-  (native_ite (__smtx_type_wf T) U SmtType.None)
+  (native_ite (native_inhabited_type T) (native_ite (__smtx_type_wf T) U SmtType.None) SmtType.None)
 
 def __smtx_msm_get_default : SmtMap -> SmtValue
   | (SmtMap.cons j e m) => (__smtx_msm_get_default m)
@@ -617,6 +617,11 @@ def __smtx_mss_op_internal (isInter : native_Bool) : SmtMap -> SmtMap -> SmtMap 
 
 def __smtx_map_to_set_type : SmtType -> SmtType
   | (SmtType.Map T SmtType.Bool) => (SmtType.Set T)
+  | T => SmtType.None
+
+
+def __smtx_map_to_fun_type : SmtType -> SmtType
+  | (SmtType.Map T U) => (SmtType.FunType T U)
   | T => SmtType.None
 
 
@@ -702,8 +707,10 @@ def __smtx_typeof_value : SmtValue -> SmtType
   | (SmtValue.RegLan r) => SmtType.RegLan
   | (SmtValue.Map m) => (__smtx_typeof_map_value m)
   | (SmtValue.Set m) => (__smtx_map_to_set_type (__smtx_typeof_map_value m))
+  | (SmtValue.Fun m) => (__smtx_map_to_fun_type (__smtx_typeof_map_value m))
   | (SmtValue.Seq ss) => (__smtx_typeof_seq_value ss)
   | (SmtValue.Char c) => SmtType.Char
+  | (SmtValue.UValue i e) => (SmtType.USort i)
   | (SmtValue.DtCons s d i) => 
     let _v0 := (SmtType.Datatype s d)
     (native_ite (__smtx_type_wf _v0) (__smtx_typeof_dt_cons_value_rec _v0 (__smtx_dt_substitute s d d) i) SmtType.None)
@@ -787,7 +794,7 @@ def __smtx_model_eval_apply : SmtValue -> SmtValue -> SmtValue
   | v, SmtValue.NotValue => SmtValue.NotValue
   | (SmtValue.DtCons s d n), i => (SmtValue.Apply (SmtValue.DtCons s d n) i)
   | (SmtValue.Apply f v), i => (SmtValue.Apply (SmtValue.Apply f v) i)
-  | (SmtValue.Map m), i => (__smtx_map_select (SmtValue.Map m) i)
+  | (SmtValue.Fun m), i => (__smtx_map_select (SmtValue.Map m) i)
   | v, i => SmtValue.NotValue
 
 
@@ -1398,7 +1405,6 @@ def __smtx_typeof_eq (T : SmtType) (U : SmtType) : SmtType :=
   (__smtx_typeof_guard T (native_ite (native_Teq T U) SmtType.Bool SmtType.None))
 
 def __smtx_typeof_apply : SmtType -> SmtType -> SmtType
-  | (SmtType.Map T U), V => (__smtx_typeof_guard T (native_ite (native_Teq T V) U SmtType.None))
   | (SmtType.FunType T U), V => (__smtx_typeof_guard T (native_ite (native_Teq T V) U SmtType.None))
   | T, U => SmtType.None
 
@@ -1646,7 +1652,7 @@ def __smtx_typeof : SmtTerm -> SmtType
   | (SmtTerm.bvusubo x1 x2) => (__smtx_typeof_bv_op_2_ret (__smtx_typeof x1) (__smtx_typeof x2) SmtType.Bool)
   | (SmtTerm.bvssubo x1 x2) => (__smtx_typeof_bv_op_2_ret (__smtx_typeof x1) (__smtx_typeof x2) SmtType.Bool)
   | (SmtTerm.bvsdivo x1 x2) => (__smtx_typeof_bv_op_2_ret (__smtx_typeof x1) (__smtx_typeof x2) SmtType.Bool)
-  | (SmtTerm.seq_empty x1) => (__smtx_typeof_guard_inhabited x1 (SmtType.Seq x1))
+  | (SmtTerm.seq_empty x1) => (__smtx_typeof_guard_wf x1 (SmtType.Seq x1))
   | (SmtTerm.str_len x1) => (__smtx_typeof_seq_op_1_ret (__smtx_typeof x1) SmtType.Int)
   | (SmtTerm.str_concat x1 x2) => (__smtx_typeof_seq_op_2 (__smtx_typeof x1) (__smtx_typeof x2))
   | (SmtTerm.str_substr x1 x2 x3) => (__smtx_typeof_str_substr (__smtx_typeof x1) (__smtx_typeof x2) (__smtx_typeof x3))
@@ -1709,7 +1715,7 @@ def __smtx_typeof : SmtTerm -> SmtType
     let _v0 := (__smtx_typeof x1)
     (native_ite (native_Teq _v0 SmtType.None) SmtType.None (SmtType.Seq _v0))
   | (SmtTerm.seq_nth x1 x2) => (__smtx_typeof_seq_nth (__smtx_typeof x1) (__smtx_typeof x2))
-  | (SmtTerm.set_empty x1) => (__smtx_typeof_guard_inhabited x1 (SmtType.Set x1))
+  | (SmtTerm.set_empty x1) => (__smtx_typeof_guard_wf x1 (SmtType.Set x1))
   | (SmtTerm.set_singleton x1) => 
     let _v0 := (__smtx_typeof x1)
     (native_ite (native_Teq _v0 SmtType.None) SmtType.None (SmtType.Set _v0))
@@ -1727,15 +1733,17 @@ def __smtx_typeof : SmtTerm -> SmtType
   | (SmtTerm.Apply (SmtTerm.Apply SmtTerm.eq x1) x2) => (__smtx_typeof_eq (__smtx_typeof x1) (__smtx_typeof x2))
   | (SmtTerm.Apply (SmtTerm.exists s T) x1) => (native_ite (native_Teq (__smtx_typeof x1) SmtType.Bool) SmtType.Bool SmtType.None)
   | (SmtTerm.Apply (SmtTerm.forall s T) x1) => (native_ite (native_Teq (__smtx_typeof x1) SmtType.Bool) SmtType.Bool SmtType.None)
-  | (SmtTerm.Apply (SmtTerm.choice s T) x1) => (native_ite (native_Teq (__smtx_typeof x1) SmtType.Bool) (__smtx_typeof_guard_inhabited T T) SmtType.None)
+  | (SmtTerm.Apply (SmtTerm.choice s T) x1) => (native_ite (native_Teq (__smtx_typeof x1) SmtType.Bool) (__smtx_typeof_guard_wf T T) SmtType.None)
   | (SmtTerm.DtCons s d i) => 
     let _v0 := (SmtType.Datatype s d)
     (__smtx_typeof_guard_wf _v0 (__smtx_typeof_dt_cons_rec _v0 (__smtx_dt_substitute s d d) i))
-  | (SmtTerm.Apply (SmtTerm.DtSel s d i j) x1) => (__smtx_typeof_apply (SmtType.FunType (SmtType.Datatype s d) (__smtx_ret_typeof_sel s d i j)) (__smtx_typeof x1))
+  | (SmtTerm.Apply (SmtTerm.DtSel s d i j) x1) => 
+    let _v0 := (__smtx_ret_typeof_sel s d i j)
+    (__smtx_typeof_guard_wf _v0 (__smtx_typeof_apply (SmtType.FunType (SmtType.Datatype s d) _v0) (__smtx_typeof x1)))
   | (SmtTerm.Apply (SmtTerm.DtTester s d i) x1) => (__smtx_typeof_apply (SmtType.FunType (SmtType.Datatype s d) SmtType.Bool) (__smtx_typeof x1))
   | (SmtTerm.Apply f x1) => (__smtx_typeof_apply (__smtx_typeof f) (__smtx_typeof x1))
-  | (SmtTerm.Var s T) => (__smtx_typeof_guard_inhabited T T)
-  | (SmtTerm.UConst s T) => (__smtx_typeof_guard_inhabited T T)
+  | (SmtTerm.Var s T) => (__smtx_typeof_guard_wf T T)
+  | (SmtTerm.UConst s T) => (__smtx_typeof_guard_wf T T)
   | x1 => SmtType.None
 
 
@@ -1900,17 +1908,17 @@ noncomputable def __smtx_model_eval (M : SmtModel) : SmtTerm -> SmtValue
   | (SmtTerm.div x1 x2) => 
     let _v0 := (__smtx_model_eval M x2)
     let _v1 := (__smtx_model_eval M x1)
-    (__smtx_model_eval_ite (__smtx_model_eval_eq _v0 (SmtValue.Numeral 0)) (__smtx_model_eval_apply (__smtx_model_lookup M native_div_by_zero_id (SmtType.Map SmtType.Int SmtType.Int)) _v1) (__smtx_model_eval_div_total _v1 _v0))
+    (__smtx_model_eval_ite (__smtx_model_eval_eq _v0 (SmtValue.Numeral 0)) (__smtx_model_eval_apply (__smtx_model_lookup M native_div_by_zero_id (SmtType.FunType SmtType.Int SmtType.Int)) _v1) (__smtx_model_eval_div_total _v1 _v0))
   | (SmtTerm.mod x1 x2) => 
     let _v0 := (__smtx_model_eval M x2)
     let _v1 := (__smtx_model_eval M x1)
-    (__smtx_model_eval_ite (__smtx_model_eval_eq _v0 (SmtValue.Numeral 0)) (__smtx_model_eval_apply (__smtx_model_lookup M native_mod_by_zero_id (SmtType.Map SmtType.Int SmtType.Int)) _v1) (__smtx_model_eval_mod_total _v1 _v0))
+    (__smtx_model_eval_ite (__smtx_model_eval_eq _v0 (SmtValue.Numeral 0)) (__smtx_model_eval_apply (__smtx_model_lookup M native_mod_by_zero_id (SmtType.FunType SmtType.Int SmtType.Int)) _v1) (__smtx_model_eval_mod_total _v1 _v0))
   | (SmtTerm.multmult x1 x2) => 
     let _v0 := (__smtx_model_eval M x2)
     let _v1 := (SmtValue.Numeral 0)
     let _v2 := (__smtx_model_eval M x1)
     let _v3 := (SmtValue.Numeral 1)
-    (__smtx_model_eval_ite (__smtx_model_eval_geq _v0 _v1) (__smtx_model_eval_multmult_total _v2 _v0) (__smtx_model_eval_ite (__smtx_model_eval_eq _v2 _v1) (__smtx_model_eval_apply (__smtx_model_lookup M native_div_by_zero_id (SmtType.Map SmtType.Int SmtType.Int)) _v3) (__smtx_model_eval_div_total _v3 (__smtx_model_eval_multmult_total _v2 (__smtx_model_eval__ _v1 _v0)))))
+    (__smtx_model_eval_ite (__smtx_model_eval_geq _v0 _v1) (__smtx_model_eval_multmult_total _v2 _v0) (__smtx_model_eval_ite (__smtx_model_eval_eq _v2 _v1) (__smtx_model_eval_apply (__smtx_model_lookup M native_div_by_zero_id (SmtType.FunType SmtType.Int SmtType.Int)) _v3) (__smtx_model_eval_div_total _v3 (__smtx_model_eval_multmult_total _v2 (__smtx_model_eval__ _v1 _v0)))))
   | (SmtTerm.divisible x1 x2) => (__smtx_model_eval_divisible (__smtx_model_eval M x1) (__smtx_model_eval M x2))
   | (SmtTerm.int_pow2 x1) => (__smtx_model_eval_int_pow2 (__smtx_model_eval M x1))
   | (SmtTerm.int_log2 x1) => (__smtx_model_eval_int_log2 (__smtx_model_eval M x1))
@@ -2017,7 +2025,7 @@ noncomputable def __smtx_model_eval (M : SmtModel) : SmtTerm -> SmtValue
   | (SmtTerm.qdiv x1 x2) => 
     let _v0 := (__smtx_model_eval M x2)
     let _v1 := (__smtx_model_eval M x1)
-    (__smtx_model_eval_ite (__smtx_model_eval_eq _v0 (SmtValue.Rational (native_mk_rational 0 1))) (__smtx_model_eval_apply (__smtx_model_lookup M native_qdiv_by_zero_id (SmtType.Map SmtType.Real SmtType.Real)) _v1) (__smtx_model_eval_qdiv_total _v1 _v0))
+    (__smtx_model_eval_ite (__smtx_model_eval_eq _v0 (SmtValue.Rational (native_mk_rational 0 1))) (__smtx_model_eval_apply (__smtx_model_lookup M native_qdiv_by_zero_id (SmtType.FunType SmtType.Real SmtType.Real)) _v1) (__smtx_model_eval_qdiv_total _v1 _v0))
   | (SmtTerm.qdiv_total x1 x2) => (__smtx_model_eval_qdiv_total (__smtx_model_eval M x1) (__smtx_model_eval M x2))
   | (SmtTerm.int_to_bv x1 x2) => (__smtx_model_eval_int_to_bv (__smtx_model_eval M x1) (__smtx_model_eval M x2))
   | (SmtTerm.ubv_to_int x1) => (__smtx_model_eval_ubv_to_int (__smtx_model_eval M x1))
